reworked select_inputs to omit k

Experiments/Backwards_Reachability_Analysis.thy
@@ -4,78 +4,130 @@ begin
 
 
 
-fun select_inputs :: "(('a \<times> 'b) \<Rightarrow> ('c \<times> 'a) set) \<Rightarrow> 'a \<Rightarrow> 'b list \<Rightarrow> 'a list \<Rightarrow> 'a set \<Rightarrow> nat \<Rightarrow> ('a \<times> 'b) list \<Rightarrow> ('a \<times> 'b) list" where
-  "select_inputs f q0 inputList nodeList nodeSet 0 m = (case find (\<lambda> x . f (q0,x) \<noteq> {} \<and> (\<forall> (y,q'') \<in> f (q0,x) . (q'' \<in> nodeSet))) inputList of 
+lemma remove1_length : "x \<in> set xs \<Longrightarrow> length (remove1 x xs) < length xs" 
+  by (induction xs; auto)
+
+
+function select_inputs :: "(('a \<times> 'b) \<Rightarrow> ('c \<times> 'a) set) \<Rightarrow> 'a \<Rightarrow> 'b list \<Rightarrow> 'a list \<Rightarrow> 'a set \<Rightarrow> ('a \<times> 'b) list \<Rightarrow> ('a \<times> 'b) list" where
+  "select_inputs f q0 inputList [] nodeSet m = (case find (\<lambda> x . f (q0,x) \<noteq> {} \<and> (\<forall> (y,q'') \<in> f (q0,x) . (q'' \<in> nodeSet))) inputList of 
       Some x \<Rightarrow> m@[(q0,x)] |
       None   \<Rightarrow> m)" |
-  "select_inputs f q0 inputList nodeList nodeSet (Suc k) m = 
+  "select_inputs f q0 inputList (n#nL) nodeSet m = 
     (case find (\<lambda> x . f (q0,x) \<noteq> {} \<and> (\<forall> (y,q'') \<in> f (q0,x) . (q'' \<in> nodeSet))) inputList of 
       Some x \<Rightarrow> m@[(q0,x)] |
-      None   \<Rightarrow> (case find_remove_2 (\<lambda> q' x . f (q',x) \<noteq> {} \<and> (\<forall> (y,q'') \<in> f (q',x) . (q'' \<in> nodeSet))) nodeList inputList
+      None   \<Rightarrow> (case find_remove_2 (\<lambda> q' x . f (q',x) \<noteq> {} \<and> (\<forall> (y,q'') \<in> f (q',x) . (q'' \<in> nodeSet))) (n#nL) inputList
           of None            \<Rightarrow> m |
-             Some (q',x,nodeList') \<Rightarrow> select_inputs f q0 inputList nodeList' (insert q' nodeSet) k (m@[(q',x)])))"
+             Some (q',x,nodeList') \<Rightarrow> select_inputs f q0 inputList nodeList' (insert q' nodeSet) (m@[(q',x)])))"
+  by pat_completeness auto
+termination 
+apply (relation "measure (\<lambda> (f,q0,iL,nL,nS,m) . length nL)")
+ apply simp
+proof -
+  fix f :: "(('a \<times> 'b) \<Rightarrow> ('c \<times> 'a) set)"
+  fix q0 :: 'a
+  fix inputList :: "'b list"
+  fix n :: 'a
+  fix nL :: "'a list" 
+  fix nodeSet :: "'a set"
+  fix m :: "('a \<times> 'b) list" 
+  fix qynL' q ynL' x nL'
+  assume "find (\<lambda>x. f (q0, x) \<noteq> {} \<and> (\<forall>(y, q'')\<in>f (q0, x). q'' \<in> nodeSet)) inputList = None"
+     and "find_remove_2 (\<lambda>q' x. f (q', x) \<noteq> {} \<and> (\<forall>(y, q'')\<in>f (q', x). q'' \<in> nodeSet)) (n # nL) inputList = Some qynL'"
+     and "(q, ynL') = qynL'"
+     and "(x, nL') = ynL'"
+
+  then have *: "find_remove_2 (\<lambda>q' x. f (q', x) \<noteq> {} \<and> (\<forall>(y, q'')\<in>f (q', x). q'' \<in> nodeSet)) (n # nL) inputList = Some (q,x,nL')"
+    by auto
+
+  have "q \<in> set (n # nL)"
+  and  "nL' = remove1 q (n # nL)"
+    using find_remove_2_set(2,6)[OF *] by simp+
+
+  then have "length nL' < length (n # nL)"
+    using remove1_length by metis
+    
+
+  then show "((f, q0, inputList, nL', insert q nodeSet, m @ [(q, x)]), f, q0, inputList, n # nL, nodeSet, m) \<in> measure (\<lambda>(f, q0, iL, nL, nS, m). length nL)"
+    by auto
+qed
+
+
 
 
 lemma select_inputs_length :
-  "length (select_inputs f q0 inputList nodeList nodeSet k m) \<le> (length m) + Suc k"
-proof (induction k arbitrary: nodeList nodeSet m)
+  "length (select_inputs f q0 inputList nodeList nodeSet m) \<le> (length m) + Suc (length nodeList)"
+proof (induction "length nodeList" arbitrary: nodeList nodeSet m)
   case 0
   then show ?case by (cases "find (\<lambda>x. f (q0, x) \<noteq> {} \<and> (\<forall>(y, q'')\<in>f (q0, x). q'' \<in> nodeSet)) inputList"; auto)
 next
   case (Suc k)
-  then show ?case proof (cases "find (\<lambda> x . f (q0,x) \<noteq> {} \<and> (\<forall> (y,q'') \<in> f (q0,x) . (q'' \<in> nodeSet))) inputList")
+  then obtain n nL where "nodeList = n # nL"
+    by (meson Suc_length_conv) 
+
+  show ?case proof (cases "find (\<lambda> x . f (q0,x) \<noteq> {} \<and> (\<forall> (y,q'') \<in> f (q0,x) . (q'' \<in> nodeSet))) inputList")
     case None
     then show ?thesis proof (cases "find_remove_2 (\<lambda> q' x . f (q',x) \<noteq> {} \<and> (\<forall> (y,q'') \<in> f (q',x) . (q'' \<in> nodeSet))) nodeList inputList")
       case None
-      then show ?thesis using \<open>find (\<lambda>x. f (q0, x) \<noteq> {} \<and> (\<forall>(y, q'')\<in>f (q0, x). q'' \<in> nodeSet)) inputList = None\<close> by auto
+      then show ?thesis using \<open>find (\<lambda>x. f (q0, x) \<noteq> {} \<and> (\<forall>(y, q'')\<in>f (q0, x). q'' \<in> nodeSet)) inputList = None\<close> unfolding \<open>nodeList = n # nL\<close> by auto
     next
       case (Some a)
-      then obtain q' x nodeList' where *: "find_remove_2 (\<lambda> q' x . f (q',x) \<noteq> {} \<and> (\<forall> (y,q'') \<in> f (q',x) . (q'' \<in> nodeSet))) nodeList inputList = Some (q',x,nodeList')"
-        by (metis prod_cases3)
+      then obtain q' x nodeList' where *: "find_remove_2 (\<lambda> q' x . f (q',x) \<noteq> {} \<and> (\<forall> (y,q'') \<in> f (q',x) . (q'' \<in> nodeSet))) (n#nL) inputList = Some (q',x,nodeList')"
+        unfolding \<open>nodeList = n # nL\<close> by (metis prod_cases3)
+      have "k = length nodeList'"
+        using find_remove_2_length[OF *] \<open>Suc k = length nodeList\<close> unfolding \<open>nodeList = n # nL\<close>
+        by simp
       show ?thesis 
-        unfolding select_inputs.simps None *
-        using Suc.IH[of nodeList' "insert q' nodeSet" "m@[(q',x)]"] by auto
+        unfolding \<open>nodeList = n # nL\<close> select_inputs.simps None *
+        using Suc.hyps(1)[of nodeList' "insert q' nodeSet" "m@[(q',x)]", OF \<open>k = length nodeList'\<close>] unfolding find_remove_2_length[OF *] by simp
     qed
   next
     case (Some a)
-    then show ?thesis by auto
+    then show ?thesis unfolding \<open>nodeList = n # nL\<close> by auto
   qed
 qed
 
+
 lemma select_inputs_length_min :
-  "length (select_inputs f q0 inputList nodeList nodeSet k m) \<ge> (length m)"
-proof (induction k arbitrary: nodeList nodeSet m)
+  "length (select_inputs f q0 inputList nodeList nodeSet m) \<ge> (length m)"
+proof (induction "length nodeList" arbitrary: nodeList nodeSet m)
   case 0
   then show ?case by (cases "find (\<lambda>x. f (q0, x) \<noteq> {} \<and> (\<forall>(y, q'')\<in>f (q0, x). q'' \<in> nodeSet)) inputList"; auto)
 next
   case (Suc k)
-  then show ?case proof (cases "find (\<lambda> x . f (q0,x) \<noteq> {} \<and> (\<forall> (y,q'') \<in> f (q0,x) . (q'' \<in> nodeSet))) inputList")
+  then obtain n nL where "nodeList = n # nL"
+    by (meson Suc_length_conv) 
+
+  show ?case proof (cases "find (\<lambda> x . f (q0,x) \<noteq> {} \<and> (\<forall> (y,q'') \<in> f (q0,x) . (q'' \<in> nodeSet))) inputList")
     case None
     then show ?thesis proof (cases "find_remove_2 (\<lambda> q' x . f (q',x) \<noteq> {} \<and> (\<forall> (y,q'') \<in> f (q',x) . (q'' \<in> nodeSet))) nodeList inputList")
       case None
-      then show ?thesis using \<open>find (\<lambda>x. f (q0, x) \<noteq> {} \<and> (\<forall>(y, q'')\<in>f (q0, x). q'' \<in> nodeSet)) inputList = None\<close> by auto
+      then show ?thesis using \<open>find (\<lambda>x. f (q0, x) \<noteq> {} \<and> (\<forall>(y, q'')\<in>f (q0, x). q'' \<in> nodeSet)) inputList = None\<close> unfolding \<open>nodeList = n # nL\<close> by auto
     next
       case (Some a)
-      then obtain q' x nodeList' where *: "find_remove_2 (\<lambda> q' x . f (q',x) \<noteq> {} \<and> (\<forall> (y,q'') \<in> f (q',x) . (q'' \<in> nodeSet))) nodeList inputList = Some (q',x,nodeList')"
-        by (metis prod_cases3)
+      then obtain q' x nodeList' where *: "find_remove_2 (\<lambda> q' x . f (q',x) \<noteq> {} \<and> (\<forall> (y,q'') \<in> f (q',x) . (q'' \<in> nodeSet))) (n#nL) inputList = Some (q',x,nodeList')"
+        unfolding \<open>nodeList = n # nL\<close> by (metis prod_cases3)
+      have "k = length nodeList'"
+        using find_remove_2_length[OF *] \<open>Suc k = length nodeList\<close> unfolding \<open>nodeList = n # nL\<close>
+        by simp
       show ?thesis 
-        unfolding select_inputs.simps None *
-        using Suc.IH[of "m@[(q',x)]" nodeList' "insert q' nodeSet" ] by auto
+        unfolding \<open>nodeList = n # nL\<close> select_inputs.simps None *
+        using Suc.hyps(1)[of nodeList' "m@[(q',x)]" "insert q' nodeSet" , OF \<open>k = length nodeList'\<close>] unfolding find_remove_2_length[OF *] by simp
     qed
   next
     case (Some a)
-    then show ?thesis by auto
+    then show ?thesis unfolding \<open>nodeList = n # nL\<close> by auto
   qed
 qed
+
 
 
 lemma select_inputs_helper1 :
-  "find (\<lambda>x. f (q0, x) \<noteq> {} \<and> (\<forall>(y, q'')\<in>f (q0, x). q'' \<in> nS)) iL = Some x \<Longrightarrow> (select_inputs f q0 iL nL nS k m) = m@[(q0,x)]" 
-  by (cases k; auto)
+  "find (\<lambda>x. f (q0, x) \<noteq> {} \<and> (\<forall>(y, q'')\<in>f (q0, x). q'' \<in> nS)) iL = Some x \<Longrightarrow> (select_inputs f q0 iL nL nS m) = m@[(q0,x)]" 
+  by (cases nL; auto)
 
 
 
-
+(*
 lemma select_inputs_next :
   "\<exists> m' . (select_inputs f q0 iL nL nS (Suc k) m) = (select_inputs f q0 iL nL nS k m)@m'" 
 proof (cases "find (\<lambda> x . f (q0,x) \<noteq> {} \<and> (\<forall> (y,q'') \<in> f (q0,x) . (q'' \<in> nS))) iL")
@@ -125,7 +177,7 @@ next
   show ?thesis using select_inputs_helper1[OF Some]
     by (metis append_Nil2) 
 qed
-  
+
 
 
 
@@ -165,42 +217,49 @@ lemma select_inputs_prefix_ex :
   assumes "i \<le> k"
   shows "\<exists> m' . (select_inputs f q0 iL nL nS k m) = (select_inputs f q0 iL nL nS i m) @ m'" 
   using select_inputs_prefix[OF assms] by (metis (no_types) append_take_drop_id)
-
+*)  
 
 lemma select_inputs_take :
-  "take (length m) (select_inputs f q0 iL nL nS k m) = m"
-proof (induction k arbitrary: nL nS m)
+  "take (length m) (select_inputs f q0 inputList nodeList nodeSet m) = m"
+proof (induction "length nodeList" arbitrary: nodeList nodeSet m)
   case 0
-  then show ?case by (cases "find (\<lambda>x. f (q0, x) \<noteq> {} \<and> (\<forall>(y, q'')\<in>f (q0, x). q'' \<in> nS)) iL"; auto)
+  then show ?case by (cases "find (\<lambda>x. f (q0, x) \<noteq> {} \<and> (\<forall>(y, q'')\<in>f (q0, x). q'' \<in> nodeSet)) inputList"; auto)
 next
   case (Suc k)
-  then show ?case proof (cases "find (\<lambda> x . f (q0,x) \<noteq> {} \<and> (\<forall> (y,q'') \<in> f (q0,x) . (q'' \<in> nS))) iL")
+  then obtain n nL where "nodeList = n # nL"
+    by (meson Suc_length_conv) 
+
+  show ?case proof (cases "find (\<lambda> x . f (q0,x) \<noteq> {} \<and> (\<forall> (y,q'') \<in> f (q0,x) . (q'' \<in> nodeSet))) inputList")
     case None
-    then show ?thesis proof (cases "find_remove_2 (\<lambda> q' x . f (q',x) \<noteq> {} \<and> (\<forall> (y,q'') \<in> f (q',x) . (q'' \<in> nS))) nL iL")
+    then show ?thesis proof (cases "find_remove_2 (\<lambda> q' x . f (q',x) \<noteq> {} \<and> (\<forall> (y,q'') \<in> f (q',x) . (q'' \<in> nodeSet))) nodeList inputList")
       case None
-      then show ?thesis using \<open>find (\<lambda>x. f (q0, x) \<noteq> {} \<and> (\<forall>(y, q'')\<in>f (q0, x). q'' \<in> nS)) iL = None\<close> by auto
+      then show ?thesis using \<open>find (\<lambda>x. f (q0, x) \<noteq> {} \<and> (\<forall>(y, q'')\<in>f (q0, x). q'' \<in> nodeSet)) inputList = None\<close> unfolding \<open>nodeList = n # nL\<close> by auto
     next
       case (Some a)
-      then obtain q' x nodeList' where *: "find_remove_2 (\<lambda> q' x . f (q',x) \<noteq> {} \<and> (\<forall> (y,q'') \<in> f (q',x) . (q'' \<in> nS))) nL iL = Some (q',x,nodeList')"
-        by (metis prod_cases3)
+      then obtain q' x nodeList' where *: "find_remove_2 (\<lambda> q' x . f (q',x) \<noteq> {} \<and> (\<forall> (y,q'') \<in> f (q',x) . (q'' \<in> nodeSet))) (n#nL) inputList = Some (q',x,nodeList')"
+        unfolding \<open>nodeList = n # nL\<close> by (metis prod_cases3)
+      have "k = length nodeList'"
+        using find_remove_2_length[OF *] \<open>Suc k = length nodeList\<close> unfolding \<open>nodeList = n # nL\<close>
+        by simp
 
-      have scheme: "\<And> xs ys y . take (length (ys@y)) xs = ys@y \<Longrightarrow> take (length ys) xs = ys"
-        by (metis append.assoc append_eq_conv_conj) 
-      have "take (length (m @ [(q', x)])) (select_inputs f q0 iL nL nS (Suc k) m) = (m @ [(q', x)])"
-        unfolding select_inputs.simps None *
-        using Suc.IH[of "m@[(q',x)]" nodeList' "insert q' nS" ] by auto
-      then show ?thesis
-        unfolding select_inputs.simps None * 
-        using scheme[of m "[(q',x)]"] by force
+      have **: "(select_inputs f q0 inputList nodeList nodeSet m) = select_inputs f q0 inputList nodeList' (insert q' nodeSet) (m @ [(q', x)])"
+        unfolding \<open>nodeList = n # nL\<close> select_inputs.simps None * by simp
+      show ?thesis
+        unfolding **
+        using Suc.hyps(1)[of nodeList' "m@[(q',x)]" "insert q' nodeSet" , OF \<open>k = length nodeList'\<close>] unfolding find_remove_2_length[OF *]
+        by (metis butlast_snoc butlast_take diff_Suc_1 length_append_singleton select_inputs_length_min) 
     qed
   next
     case (Some a)
-    then show ?thesis by auto
+    then show ?thesis unfolding \<open>nodeList = n # nL\<close> by auto
   qed
 qed
 
+
+
+
 lemma select_inputs_take' :
-  "take (length m) (select_inputs f q0 iL nL nS k (m@m')) = m"
+  "take (length m) (select_inputs f q0 iL nL nS (m@m')) = m"
   using select_inputs_take
   by (metis (no_types, lifting) add_leE append_eq_append_conv select_inputs_length_min length_append length_take min_absorb2 take_add)
 
@@ -213,23 +272,34 @@ lemma select_inputs_distinct :
   and     "distinct nL"
   and     "q0 \<notin> set nL"
   and     "set nL \<inter> nS = {}"
-  shows "distinct (map fst (select_inputs f q0 iL nL nS k m))" 
-using assms proof (induction k arbitrary: nL nS m)
+  shows "distinct (map fst (select_inputs f q0 iL nL nS m))" 
+using assms proof (induction "length nL" arbitrary: nL nS m)
   case 0
   then show ?case by (cases "find (\<lambda>x. f (q0, x) \<noteq> {} \<and> (\<forall>(y, q'')\<in>f (q0, x). q'' \<in> nS)) iL"; auto)
 next
   case (Suc k)
-  then show ?case proof (cases "find (\<lambda> x . f (q0,x) \<noteq> {} \<and> (\<forall> (y,q'') \<in> f (q0,x) . (q'' \<in> nS))) iL")
+  then obtain n nL'' where "nL = n # nL''"
+    by (meson Suc_length_conv) 
+
+  show ?case proof (cases "find (\<lambda> x . f (q0,x) \<noteq> {} \<and> (\<forall> (y,q'') \<in> f (q0,x) . (q'' \<in> nS))) iL")
     case None
     then show ?thesis proof (cases "find_remove_2 (\<lambda> q' x . f (q',x) \<noteq> {} \<and> (\<forall> (y,q'') \<in> f (q',x) . (q'' \<in> nS))) nL iL")
       case None
-      then have "(select_inputs f q0 iL nL nS (Suc k) m) = m"
-        using \<open>find (\<lambda>x. f (q0, x) \<noteq> {} \<and> (\<forall>(y, q'')\<in>f (q0, x). q'' \<in> nS)) iL = None\<close> by auto
+      then have "(select_inputs f q0 iL nL nS m) = m"
+        using \<open>find (\<lambda>x. f (q0, x) \<noteq> {} \<and> (\<forall>(y, q'')\<in>f (q0, x). q'' \<in> nS)) iL = None\<close> unfolding \<open>nL = n # nL''\<close> by auto
       then show ?thesis using Suc.prems by auto
     next
       case (Some a)
       then obtain q' x nL' where *: "find_remove_2 (\<lambda> q' x . f (q',x) \<noteq> {} \<and> (\<forall> (y,q'') \<in> f (q',x) . (q'' \<in> nS))) nL iL = Some (q',x,nL')"
         by (metis prod_cases3)
+
+      have "k = length nL'"
+        using find_remove_2_length[OF *] \<open>Suc k = length nL\<close> by simp
+
+      have "select_inputs f q0 iL nL nS m = select_inputs f q0 iL nL' (insert q' nS) (m @ [(q', x)])" 
+        using *
+        unfolding  \<open>nL = n # nL''\<close> select_inputs.simps None by auto
+
 
       have "q' \<in> set nL"
       and  "set nL' = set nL - {q'}"
@@ -251,16 +321,17 @@ next
 
       show ?thesis 
         unfolding select_inputs.simps None *
-        using Suc.IH[OF \<open>distinct (map fst (m@[(q',x)]))\<close>
-                        \<open>set (map fst (m@[(q',x)])) \<subseteq> insert q' nS\<close>
-                        \<open>q0 \<notin> insert q' nS\<close>
-                        \<open>distinct nL'\<close>
-                        \<open>q0 \<notin> set nL'\<close>
-                        \<open>set nL' \<inter> insert q' nS = {}\<close>] by auto
+        using Suc.hyps(1)[OF \<open>k = length nL'\<close> \<open>distinct (map fst (m@[(q',x)]))\<close>
+                               \<open>set (map fst (m@[(q',x)])) \<subseteq> insert q' nS\<close>
+                               \<open>q0 \<notin> insert q' nS\<close>
+                               \<open>distinct nL'\<close>
+                               \<open>q0 \<notin> set nL'\<close>
+                               \<open>set nL' \<inter> insert q' nS = {}\<close>]
+        unfolding \<open>select_inputs f q0 iL nL nS m = select_inputs f q0 iL nL' (insert q' nS) (m @ [(q', x)])\<close> by assumption
     qed
   next
     case (Some a)
-    then show ?thesis using Suc by auto
+    then show ?thesis using Suc \<open>nL = n # nL''\<close> by auto
   qed
 qed
 
@@ -268,7 +339,7 @@ qed
 
 
 lemma select_inputs_index_properties : 
-  assumes "i < length (select_inputs (h M) q0 iL nL nS k m)"
+  assumes "i < length (select_inputs (h M) q0 iL nL nS m)"
   and     "i \<ge> length m"
   and     "distinct (map fst m)"
   and     "nS = nS0 \<union> set (map fst m)"
@@ -276,72 +347,80 @@ lemma select_inputs_index_properties :
   and     "distinct nL"
   and     "q0 \<notin> set nL"
   and     "set nL \<inter> nS = {}"
-shows "fst (select_inputs (h M) q0 iL nL nS k m ! i) \<in> (insert q0 (set nL))" 
-      "fst (select_inputs (h M) q0 iL nL nS k m ! i) \<notin> nS0"
-      "snd (select_inputs (h M) q0 iL nL nS k m ! i) \<in> set iL"
-      "(\<forall> qx' \<in> set (take i (select_inputs (h M) q0 iL nL nS k m)) . fst (select_inputs (h M) q0 iL nL nS k m ! i) \<noteq> fst qx')"
-      "(\<exists> t \<in> transitions M . t_source t = fst (select_inputs (h M) q0 iL nL nS k m ! i) \<and> t_input t = snd (select_inputs (h M) q0 iL nL nS k m ! i))"
-      "(\<forall> t \<in> transitions M . (t_source t = fst (select_inputs (h M) q0 iL nL nS k m ! i) \<and> t_input t = snd (select_inputs (h M) q0 iL nL nS k m ! i)) \<longrightarrow> (t_target t \<in> nS0 \<or> (\<exists> qx' \<in> set (take i (select_inputs (h M) q0 iL nL nS k m)) . fst qx' = (t_target t))))"
+shows "fst (select_inputs (h M) q0 iL nL nS m ! i) \<in> (insert q0 (set nL))" 
+      "fst (select_inputs (h M) q0 iL nL nS m ! i) \<notin> nS0"
+      "snd (select_inputs (h M) q0 iL nL nS m ! i) \<in> set iL"
+      "(\<forall> qx' \<in> set (take i (select_inputs (h M) q0 iL nL nS m)) . fst (select_inputs (h M) q0 iL nL nS m ! i) \<noteq> fst qx')"
+      "(\<exists> t \<in> transitions M . t_source t = fst (select_inputs (h M) q0 iL nL nS m ! i) \<and> t_input t = snd (select_inputs (h M) q0 iL nL nS m ! i))"
+      "(\<forall> t \<in> transitions M . (t_source t = fst (select_inputs (h M) q0 iL nL nS m ! i) \<and> t_input t = snd (select_inputs (h M) q0 iL nL nS m ! i)) \<longrightarrow> (t_target t \<in> nS0 \<or> (\<exists> qx' \<in> set (take i (select_inputs (h M) q0 iL nL nS m)) . fst qx' = (t_target t))))"
 proof -
   have combined_props : 
-    "fst (select_inputs (h M) q0 iL nL nS k m ! i) \<in> (insert q0 (set nL))
-      \<and> snd (select_inputs (h M) q0 iL nL nS k m ! i) \<in> set iL
-      \<and> fst (select_inputs (h M) q0 iL nL nS k m ! i) \<notin> nS0
-      \<and> (\<exists> t \<in> transitions M . t_source t = fst (select_inputs (h M) q0 iL nL nS k m ! i) \<and> t_input t = snd (select_inputs (h M) q0 iL nL nS k m ! i))
-      \<and> (\<forall> t \<in> transitions M . (t_source t = fst (select_inputs (h M) q0 iL nL nS k m ! i) \<and> t_input t = snd (select_inputs (h M) q0 iL nL nS k m ! i)) \<longrightarrow> (t_target t \<in> nS0 \<or> (\<exists> qx' \<in> set (take i (select_inputs (h M) q0 iL nL nS k m)) . fst qx' = (t_target t))))"    
-  using assms proof (induction k arbitrary: nL nS m)
+    "fst (select_inputs (h M) q0 iL nL nS m ! i) \<in> (insert q0 (set nL))
+      \<and> snd (select_inputs (h M) q0 iL nL nS m ! i) \<in> set iL
+      \<and> fst (select_inputs (h M) q0 iL nL nS m ! i) \<notin> nS0
+      \<and> (\<exists> t \<in> transitions M . t_source t = fst (select_inputs (h M) q0 iL nL nS m ! i) \<and> t_input t = snd (select_inputs (h M) q0 iL nL nS m ! i))
+      \<and> (\<forall> t \<in> transitions M . (t_source t = fst (select_inputs (h M) q0 iL nL nS m ! i) \<and> t_input t = snd (select_inputs (h M) q0 iL nL nS m ! i)) \<longrightarrow> (t_target t \<in> nS0 \<or> (\<exists> qx' \<in> set (take i (select_inputs (h M) q0 iL nL nS m)) . fst qx' = (t_target t))))"    
+  using assms proof (induction "length nL" arbitrary: nL nS m)
     case 0
     show ?case proof (cases "find (\<lambda> x . (h M) (q0,x) \<noteq> {} \<and> (\<forall> (y,q'') \<in> (h M) (q0,x) . (q'' \<in> nS))) iL")
       case None
-      then have "(select_inputs (h M) q0 iL nL nS 0 m) = m" by auto
+      then have "(select_inputs (h M) q0 iL nL nS m) = m" using 0 by auto
       then have "False" using "0.prems"(1,2) by auto
       then show ?thesis by simp
     next
       case (Some x)
-      have "(select_inputs (h M) q0 iL nL nS 0 m) = m@[(q0,x)]" using select_inputs_helper1[OF Some] by assumption
-      then have "(select_inputs (h M) q0 iL nL nS 0 m ! i) = (q0,x)" using "0.prems"(1,2)
+      have "(select_inputs (h M) q0 iL nL nS m) = m@[(q0,x)]" using select_inputs_helper1[OF Some] by assumption
+      then have "(select_inputs (h M) q0 iL nL nS m ! i) = (q0,x)" using "0.prems"(1,2)
         using antisym by fastforce 
   
       have "fst (q0, x) \<in> insert q0 (set nL)" by auto
       moreover have "snd (q0, x) \<in> set iL" using find_set[OF Some] by auto
-      moreover have "fst (select_inputs (h M) q0 iL nL nS 0 m ! i) \<notin> nS0"
-        using \<open>select_inputs (h M) q0 iL nL nS 0 m ! i = (q0, x)\<close> assms(4) assms(5) by auto
+      moreover have "fst (select_inputs (h M) q0 iL nL nS m ! i) \<notin> nS0"
+        using \<open>select_inputs (h M) q0 iL nL nS m ! i = (q0, x)\<close> assms(4) assms(5) by auto
        
       moreover have "(\<exists>t\<in>FSM.transitions M. t_source t = fst (q0, x) \<and> t_input t = snd (q0, x))"
         using find_condition[OF Some] unfolding fst_conv snd_conv h.simps
         by fastforce 
       moreover have "\<And> t . t \<in> FSM.transitions M \<Longrightarrow>
           t_source t = fst (q0, x) \<Longrightarrow> t_input t = snd (q0, x) \<Longrightarrow>
-          t_target t \<in> nS0 \<or> (\<exists>qx'\<in>set (take i (select_inputs (h M) q0 iL nL nS 0 m)). fst qx' = t_target t)"   
+          t_target t \<in> nS0 \<or> (\<exists>qx'\<in>set (take i (select_inputs (h M) q0 iL nL nS m)). fst qx' = t_target t)"   
       proof -
         fix t assume "t \<in> FSM.transitions M" "t_source t = fst (q0, x)" "t_input t = snd (q0, x)"
         then have "t_target t \<in> nS"
           using find_condition[OF Some] unfolding h.simps fst_conv snd_conv
           by (metis (mono_tags, lifting) case_prod_beta' mem_Collect_eq prod.collapse) 
-        then show "t_target t \<in> nS0 \<or> (\<exists>qx'\<in>set (take i (select_inputs (h M) q0 iL nL nS 0 m)). fst qx' = t_target t)"
+        then show "t_target t \<in> nS0 \<or> (\<exists>qx'\<in>set (take i (select_inputs (h M) q0 iL nL nS m)). fst qx' = t_target t)"
           using \<open>nS = nS0 \<union> set (map fst m)\<close>
-          using "0.prems"(1) "0.prems"(2) \<open>select_inputs (h M) q0 iL nL nS 0 m = m @ [(q0, x)]\<close> by fastforce    
+          using "0.prems"(1) "0.prems"(2) \<open>select_inputs (h M) q0 iL nL nS m = m @ [(q0, x)]\<close> by fastforce    
       qed
         
       ultimately show ?thesis 
-        unfolding \<open>(select_inputs (h M) q0 iL nL nS 0 m ! i) = (q0,x)\<close> by blast
+        unfolding \<open>(select_inputs (h M) q0 iL nL nS m ! i) = (q0,x)\<close> by blast
     qed
   next
     case (Suc k)
+    then obtain n nL'' where "nL = n # nL''"
+      by (meson Suc_length_conv) 
+
     show ?case proof (cases "find (\<lambda> x . (h M) (q0,x) \<noteq> {} \<and> (\<forall> (y,q'') \<in> (h M) (q0,x) . (q'' \<in> nS))) iL")
       case None
       show ?thesis proof (cases "find_remove_2 (\<lambda> q' x . (h M) (q',x) \<noteq> {} \<and> (\<forall> (y,q'') \<in> (h M) (q',x) . (q'' \<in> nS))) nL iL")
         case None
-        then have "(select_inputs (h M) q0 iL nL nS (Suc k) m) = m" using \<open>find (\<lambda>x. h M (q0, x) \<noteq> {} \<and> (\<forall>(y, q'')\<in>h M (q0, x). q'' \<in> nS)) iL = None\<close> by auto
+        then have "(select_inputs (h M) q0 iL nL nS m) = m" using \<open>find (\<lambda>x. h M (q0, x) \<noteq> {} \<and> (\<forall>(y, q'')\<in>h M (q0, x). q'' \<in> nS)) iL = None\<close> \<open>nL = n # nL''\<close> by auto
         then have "False" using Suc.prems(1,2) by auto
         then show ?thesis by simp
       next
         case (Some a)
         then obtain q' x nL' where **: "find_remove_2 (\<lambda> q' x . (h M) (q',x) \<noteq> {} \<and> (\<forall> (y,q'') \<in> (h M) (q',x) . (q'' \<in> nS))) nL iL = Some (q',x,nL')"
           by (metis prod_cases3)
-        then have "select_inputs (h M) q0 iL nL nS (Suc k) m = select_inputs (h M) q0 iL nL' (insert q' nS) k (m@[(q',x)])"
-          using None by auto
-        then have "i < length (select_inputs (h M) q0 iL nL' (insert q' nS) k (m@[(q',x)]))"
+
+        have "k = length nL'"
+          using find_remove_2_length[OF **] \<open>Suc k = length nL\<close> by simp
+
+        have "select_inputs (h M) q0 iL nL nS m = select_inputs (h M) q0 iL nL' (insert q' nS) (m @ [(q', x)])" 
+          using **
+          unfolding  \<open>nL = n # nL''\<close> select_inputs.simps None by auto
+        then have "i < length (select_inputs (h M) q0 iL nL' (insert q' nS) (m@[(q',x)]))"
           using Suc.prems(1) by auto
 
         have "(set (map fst (m @ [(q', x)]))) \<subseteq> insert q' nS"
@@ -372,8 +451,7 @@ proof -
           case True
 
           show ?thesis
-            
-            using Suc.IH[OF \<open>i < length (select_inputs (h M) q0 iL nL' (insert q' nS) k (m@[(q',x)]))\<close>
+            using Suc.hyps(1)[OF \<open>k = length nL'\<close> \<open>i < length (select_inputs (h M) q0 iL nL' (insert q' nS) (m@[(q',x)]))\<close>
                             True
                             \<open>distinct (map fst (m @ [(q', x)]))\<close>
                             \<open>insert q' nS = nS0 \<union> set (map fst (m@[(q',x)]))\<close>
@@ -381,14 +459,14 @@ proof -
                             \<open>distinct nL'\<close>
                             \<open>q0 \<notin> set nL'\<close>
                             \<open>set nL' \<inter> insert q' nS = {}\<close> ]
-            unfolding \<open>select_inputs (h M) q0 iL nL nS (Suc k) m = select_inputs (h M) q0 iL nL' (insert q' nS) k (m@[(q',x)])\<close> 
+            unfolding \<open>select_inputs (h M) q0 iL nL nS m = select_inputs (h M) q0 iL nL' (insert q' nS) (m@[(q',x)])\<close> 
             using \<open>set nL' \<subseteq> set nL\<close> by blast
         next
           case False 
           then have "i = length m"
             using Suc.prems(2) by auto
-          then have ***: "select_inputs (h M) q0 iL nL nS (Suc k) m ! i = (q',x)"
-            unfolding \<open>select_inputs (h M) q0 iL nL nS (Suc k) m = select_inputs (h M) q0 iL nL' (insert q' nS) k (m@[(q',x)])\<close> 
+          then have ***: "select_inputs (h M) q0 iL nL nS m ! i = (q',x)"
+            unfolding \<open>select_inputs (h M) q0 iL nL nS m = select_inputs (h M) q0 iL nL' (insert q' nS) (m@[(q',x)])\<close> 
             using select_inputs_take
             by (metis length_append_singleton lessI nth_append_length nth_take) 
             
@@ -401,7 +479,7 @@ proof -
             using Suc.prems(4) Suc.prems(8) \<open>q' \<in> set nL\<close> by blast
           moreover have "(\<exists>t\<in>FSM.transitions M. t_source t = q' \<and> t_input t = x) "
             using find_remove_2_set(1)[OF ** ] unfolding h.simps by force
-          moreover have "(\<forall>t\<in>FSM.transitions M. t_source t = q' \<and> t_input t = x \<longrightarrow> t_target t \<in> nS0 \<or> (\<exists>qx'\<in>set (take i (select_inputs (h M) q0 iL nL nS (Suc k) m)). fst qx' = t_target t))"
+          moreover have "(\<forall>t\<in>FSM.transitions M. t_source t = q' \<and> t_input t = x \<longrightarrow> t_target t \<in> nS0 \<or> (\<exists>qx'\<in>set (take i (select_inputs (h M) q0 iL nL nS m)). fst qx' = t_target t))"
             unfolding \<open>i = length m\<close> select_inputs_take 
             using find_remove_2_set(1)[OF ** ] unfolding h.simps \<open>nS = nS0 \<union> (set (map fst m))\<close> by force
           ultimately show ?thesis 
@@ -410,61 +488,61 @@ proof -
       qed
     next
       case (Some x)
-      have "(select_inputs (h M) q0 iL nL nS (Suc k) m) = m@[(q0,x)]" using select_inputs_helper1[OF Some] by assumption
-      then have "(select_inputs (h M) q0 iL nL nS (Suc k) m ! i) = (q0,x)" using Suc.prems(1,2)
+      have "(select_inputs (h M) q0 iL nL nS m) = m@[(q0,x)]" using select_inputs_helper1[OF Some] by assumption
+      then have "(select_inputs (h M) q0 iL nL nS m ! i) = (q0,x)" using Suc.prems(1,2)
         using antisym by fastforce 
   
       have "fst (q0, x) \<in> insert q0 (set nL)" by auto
       moreover have "snd (q0, x) \<in> set iL" using find_set[OF Some] by auto
       moreover have "fst (q0, x) \<notin> nS0"
         using assms(4) assms(5) by auto 
-      moreover have "\<And> qx' . qx' \<in> set (take i (select_inputs (h M) q0 iL nL nS (Suc k) m)) - set (take (length m) (select_inputs (h M) q0 iL nL nS (Suc k) m)) \<Longrightarrow> fst (q0, x) \<noteq> fst qx'"
-        using Suc.prems(1,2) \<open>select_inputs (h M) q0 iL nL nS (Suc k) m = m @ [(q0, x)]\<close> by auto
+      moreover have "\<And> qx' . qx' \<in> set (take i (select_inputs (h M) q0 iL nL nS m)) - set (take (length m) (select_inputs (h M) q0 iL nL nS m)) \<Longrightarrow> fst (q0, x) \<noteq> fst qx'"
+        using Suc.prems(1,2) \<open>select_inputs (h M) q0 iL nL nS m = m @ [(q0, x)]\<close> by auto
       moreover have "(\<exists>t\<in>FSM.transitions M. t_source t = fst (q0, x) \<and> t_input t = snd (q0, x))"
         using find_condition[OF Some] unfolding fst_conv snd_conv h.simps
         by fastforce 
       moreover have "\<And> t . t \<in> FSM.transitions M \<Longrightarrow>
           t_source t = fst (q0, x) \<Longrightarrow> t_input t = snd (q0, x) \<Longrightarrow>
-          t_target t \<in> nS0 \<or> (\<exists>qx'\<in>set (take i (select_inputs (h M) q0 iL nL nS (Suc k) m)). fst qx' = t_target t)"   
+          t_target t \<in> nS0 \<or> (\<exists>qx'\<in>set (take i (select_inputs (h M) q0 iL nL nS m)). fst qx' = t_target t)"   
       proof -
         fix t assume "t \<in> FSM.transitions M" "t_source t = fst (q0, x)" "t_input t = snd (q0, x)"
         then have "t_target t \<in> nS"
           using find_condition[OF Some] unfolding h.simps fst_conv snd_conv
           by (metis (mono_tags, lifting) case_prod_beta' mem_Collect_eq prod.collapse) 
-        then show "t_target t \<in> nS0 \<or> (\<exists>qx'\<in>set (take i (select_inputs (h M) q0 iL nL nS (Suc k) m)). fst qx' = t_target t)"
+        then show "t_target t \<in> nS0 \<or> (\<exists>qx'\<in>set (take i (select_inputs (h M) q0 iL nL nS m)). fst qx' = t_target t)"
           using \<open>nS = nS0 \<union> (set (map fst m))\<close>
-          using Suc.prems(1,2) \<open>select_inputs (h M) q0 iL nL nS (Suc k) m = m @ [(q0, x)]\<close> by fastforce    
+          using Suc.prems(1,2) \<open>select_inputs (h M) q0 iL nL nS m = m @ [(q0, x)]\<close> by fastforce    
       qed
         
       ultimately show ?thesis 
-        unfolding \<open>(select_inputs (h M) q0 iL nL nS (Suc k) m ! i) = (q0,x)\<close> by blast
+        unfolding \<open>(select_inputs (h M) q0 iL nL nS m ! i) = (q0,x)\<close> by blast
     qed
   qed
 
-  then show "fst (select_inputs (h M) q0 iL nL nS k m ! i) \<in> (insert q0 (set nL))"
-            "snd (select_inputs (h M) q0 iL nL nS k m ! i) \<in> set iL"
-            "fst (select_inputs (h M) q0 iL nL nS k m ! i) \<notin> nS0"
-            "(\<exists> t \<in> transitions M . t_source t = fst (select_inputs (h M) q0 iL nL nS k m ! i) \<and> t_input t = snd (select_inputs (h M) q0 iL nL nS k m ! i))"
-            "(\<forall> t \<in> transitions M . (t_source t = fst (select_inputs (h M) q0 iL nL nS k m ! i) \<and> t_input t = snd (select_inputs (h M) q0 iL nL nS k m ! i)) \<longrightarrow> (t_target t \<in> nS0 \<or> (\<exists> qx' \<in> set (take i (select_inputs (h M) q0 iL nL nS k m)) . fst qx' = (t_target t))))"
+  then show "fst (select_inputs (h M) q0 iL nL nS m ! i) \<in> (insert q0 (set nL))"
+            "snd (select_inputs (h M) q0 iL nL nS m ! i) \<in> set iL"
+            "fst (select_inputs (h M) q0 iL nL nS m ! i) \<notin> nS0"
+            "(\<exists> t \<in> transitions M . t_source t = fst (select_inputs (h M) q0 iL nL nS m ! i) \<and> t_input t = snd (select_inputs (h M) q0 iL nL nS m ! i))"
+            "(\<forall> t \<in> transitions M . (t_source t = fst (select_inputs (h M) q0 iL nL nS m ! i) \<and> t_input t = snd (select_inputs (h M) q0 iL nL nS m ! i)) \<longrightarrow> (t_target t \<in> nS0 \<or> (\<exists> qx' \<in> set (take i (select_inputs (h M) q0 iL nL nS m)) . fst qx' = (t_target t))))"
     by blast+
 
-  show "(\<forall> qx' \<in> set (take i (select_inputs (h M) q0 iL nL nS k m)) . fst (select_inputs (h M) q0 iL nL nS k m ! i) \<noteq> fst qx')" 
+  show "(\<forall> qx' \<in> set (take i (select_inputs (h M) q0 iL nL nS m)) . fst (select_inputs (h M) q0 iL nL nS m ! i) \<noteq> fst qx')" 
   proof 
-    fix qx' assume "qx' \<in> set (take i (select_inputs (h M) q0 iL nL nS k m))"
-    then obtain j where "(take i (select_inputs (h M) q0 iL nL nS k m)) ! j = qx'" and "j < length (take i (select_inputs (h M) q0 iL nL nS k m))"
+    fix qx' assume "qx' \<in> set (take i (select_inputs (h M) q0 iL nL nS m))"
+    then obtain j where "(take i (select_inputs (h M) q0 iL nL nS m)) ! j = qx'" and "j < length (take i (select_inputs (h M) q0 iL nL nS m))"
       by (meson in_set_conv_nth)
-    then have "fst qx' = (map fst (select_inputs (h M) q0 iL nL nS k m)) ! j" and "j < length (select_inputs (h M) q0 iL nL nS k m)" by auto
+    then have "fst qx' = (map fst (select_inputs (h M) q0 iL nL nS m)) ! j" and "j < length (select_inputs (h M) q0 iL nL nS m)" by auto
       
-    moreover have "fst (select_inputs (h M) q0 iL nL nS k m ! i) = (map fst (select_inputs (h M) q0 iL nL nS k m)) ! i"
+    moreover have "fst (select_inputs (h M) q0 iL nL nS m ! i) = (map fst (select_inputs (h M) q0 iL nL nS m)) ! i"
       using assms(1) by auto
 
     moreover have "j \<noteq> i" 
-      using \<open>j < length (take i (select_inputs (h M) q0 iL nL nS k m))\<close> by auto
+      using \<open>j < length (take i (select_inputs (h M) q0 iL nL nS m))\<close> by auto
 
     moreover have "set (map fst m) \<subseteq> nS"
       using \<open>nS = nS0 \<union> set (map fst m)\<close> by blast
 
-    ultimately show "fst (select_inputs (h M) q0 iL nL nS k m ! i) \<noteq> fst qx'"
+    ultimately show "fst (select_inputs (h M) q0 iL nL nS m ! i) \<noteq> fst qx'"
       using assms(1)
       using select_inputs_distinct[OF \<open>distinct (map fst m)\<close> _ \<open>q0 \<notin> nS\<close> \<open>distinct nL\<close> \<open>q0 \<notin> set nL\<close> \<open>set nL \<inter> nS = {}\<close>]
       by (metis distinct_Ex1 in_set_conv_nth length_map)
@@ -472,7 +550,7 @@ proof -
 qed 
 
 
-
+(*
 lemma select_inputs_Suc_length :
   assumes "(select_inputs f q0 iL nL nS (Suc k) m) \<noteq> (select_inputs f q0 iL nL nS k m)"
   shows "length (select_inputs f q0 iL nL nS k m) = (length m) + k"
@@ -622,21 +700,23 @@ next
     then show ?thesis using select_inputs_Suc_length by metis
   qed
 qed
-
+*)
 
 lemma select_inputs_initial :
-  assumes "qx \<in> set (select_inputs f q0 iL nL nS k m) - set m"
+  assumes "qx \<in> set (select_inputs f q0 iL nL nS m) - set m"
   and     "fst qx = q0"
-  shows "(last (select_inputs f q0 iL nL nS k m)) = qx"
-using assms(1) proof (induction k arbitrary: nS nL m)
+  shows "(last (select_inputs f q0 iL nL nS m)) = qx"
+using assms(1) proof (induction "length nL" arbitrary: nS nL m)
   case 0
-  then have "find (\<lambda>x. f (q0, x) \<noteq> {} \<and> (\<forall>(y, q'')\<in>f (q0, x). q'' \<in> nS)) iL \<noteq> None" 
-    unfolding select_inputs.simps
-    by (metis Diff_cancel empty_iff option.simps(4)) 
+  then have "nL = []" by auto
+
+  have "find (\<lambda>x. f (q0, x) \<noteq> {} \<and> (\<forall>(y, q'')\<in>f (q0, x). q'' \<in> nS)) iL \<noteq> None" 
+    using 0 unfolding \<open>nL = []\<close> select_inputs.simps 
+    by (metis Diff_cancel empty_iff option.simps(4))
   then obtain x where *: "find (\<lambda>x. f (q0, x) \<noteq> {} \<and> (\<forall>(y, q'')\<in>f (q0, x). q'' \<in> nS)) iL = Some x" 
     by auto
   
-  have "set (select_inputs f q0 iL nL nS k m) - set m = {qx}"
+  have "set (select_inputs f q0 iL nL nS m) - set m = {qx}"
     using "0.prems"(1) unfolding select_inputs_helper1[OF *]
     by auto 
   
@@ -644,12 +724,15 @@ using assms(1) proof (induction k arbitrary: nS nL m)
     by (metis DiffD1 DiffD2 UnE empty_iff empty_set insert_iff last_snoc list.simps(15) set_append) 
 next
   case (Suc k)
+  then obtain n nL'' where "nL = n # nL''"
+    by (meson Suc_length_conv) 
+
   show ?case proof (cases "find (\<lambda>x. f (q0, x) \<noteq> {} \<and> (\<forall>(y, q'')\<in>f (q0, x). q'' \<in> nS)) iL")
     case None
     show ?thesis proof (cases "find_remove_2 (\<lambda> q' x . f (q',x) \<noteq> {} \<and> (\<forall> (y,q'') \<in> f (q',x) . (q'' \<in> nS))) nL iL")
       case None
-      have "(select_inputs f q0 iL nL nS (Suc k) m) = m"
-        using \<open>find (\<lambda>x. f (q0, x) \<noteq> {} \<and> (\<forall>(y, q'')\<in>f (q0, x). q'' \<in> nS)) iL = None\<close> None by auto
+      have "(select_inputs f q0 iL nL nS m) = m"
+        using \<open>find (\<lambda>x. f (q0, x) \<noteq> {} \<and> (\<forall>(y, q'')\<in>f (q0, x). q'' \<in> nS)) iL = None\<close> None \<open>nL = n # nL''\<close> by auto
       then have "False" 
         using Suc.prems(1)
         by simp
@@ -658,23 +741,29 @@ next
       case (Some a)
       then obtain q' x nL' where **: "find_remove_2 (\<lambda> q' x . f (q',x) \<noteq> {} \<and> (\<forall> (y,q'') \<in> f (q',x) . (q'' \<in> nS))) nL iL = Some (q',x,nL')"
         by (metis prod_cases3)
-      then have "(select_inputs f q0 iL nL nS (Suc k) m) = (select_inputs f q0 iL nL' (insert q' nS) k (m@[(q',x)]))"
-        using None by auto
-      then have "qx \<in> set (select_inputs f q0 iL nL' (insert q' nS) k (m@[(q',x)])) - set m"
+
+      have "k = length nL'"
+        using find_remove_2_length[OF **] \<open>Suc k = length nL\<close> by simp
+
+      have "select_inputs f q0 iL nL nS m = select_inputs f q0 iL nL' (insert q' nS) (m @ [(q', x)])" 
+        using **
+        unfolding  \<open>nL = n # nL''\<close> select_inputs.simps None by auto
+      then have "qx \<in> set (select_inputs f q0 iL nL' (insert q' nS) (m@[(q',x)])) - set m"
         using Suc.prems by auto
       moreover have "q0 \<noteq> q'"
         using None unfolding find_None_iff
         using find_remove_2_set(1,2,3)[OF **]
         by blast
-      ultimately have "qx \<in> set (select_inputs f q0 iL nL' (insert q' nS) k (m@[(q',x)])) - set (m@[(q',x)])"
+      ultimately have "qx \<in> set (select_inputs f q0 iL nL' (insert q' nS) (m@[(q',x)])) - set (m@[(q',x)])"
         using \<open>fst qx = q0\<close> by auto
       then show ?thesis 
-        using Suc.IH unfolding \<open>(select_inputs f q0 iL nL nS (Suc k) m) = (select_inputs f q0 iL nL' (insert q' nS) k (m@[(q',x)]))\<close> by metis
+        using Suc.hyps unfolding \<open>(select_inputs f q0 iL nL nS m) = (select_inputs f q0 iL nL' (insert q' nS) (m@[(q',x)]))\<close>
+        using \<open>k = length nL'\<close> by blast 
     qed
   next
     case (Some a)
 
-    have "set (select_inputs f q0 iL nL nS k m) - set m = {qx}"
+    have "set (select_inputs f q0 iL nL nS m ) - set m = {qx}"
       using Suc.prems(1) unfolding select_inputs_helper1[OF Some]
       by auto 
     
@@ -687,32 +776,40 @@ qed
 
 lemma select_inputs_max_length :
   assumes "distinct nL"
-  shows "length (select_inputs f q0 iL nL nS k m) \<le> length m + Suc (length nL)" 
-using assms proof (induction k arbitrary: nL nS m)
+  shows "length (select_inputs f q0 iL nL nS m) \<le> length m + Suc (length nL)" 
+using assms proof (induction "length nL" arbitrary: nL nS m)
   case 0
   then show ?case by (cases "find (\<lambda> x . f (q0,x) \<noteq> {} \<and> (\<forall> (y,q'') \<in> f (q0,x) . (q'' \<in> nS))) iL"; auto)
 next
   case (Suc k)
+  then obtain n nL'' where "nL = n # nL''"
+    by (meson Suc_length_conv) 
+
   show ?case proof (cases "find (\<lambda> x . f (q0,x) \<noteq> {} \<and> (\<forall> (y,q'') \<in> f (q0,x) . (q'' \<in> nS))) iL")
     case None
     show ?thesis proof (cases "find_remove_2 (\<lambda> q' x . f (q',x) \<noteq> {} \<and> (\<forall> (y,q'') \<in> f (q',x) . (q'' \<in> nS))) nL iL")
       case None
-      show ?thesis unfolding select_inputs.simps None \<open>find (\<lambda>x. f (q0, x) \<noteq> {} \<and> (\<forall>(y, q'')\<in>f (q0, x). q'' \<in> nS)) iL = None\<close> by auto
+      show ?thesis unfolding \<open>nL = n # nL''\<close> select_inputs.simps None \<open>find (\<lambda>x. f (q0, x) \<noteq> {} \<and> (\<forall>(y, q'')\<in>f (q0, x). q'' \<in> nS)) iL = None\<close>
+        using None \<open>nL = n # nL''\<close> by auto 
     next
       case (Some a)
       then obtain q' x nL' where **: "find_remove_2 (\<lambda> q' x . f (q',x) \<noteq> {} \<and> (\<forall> (y,q'') \<in> f (q',x) . (q'' \<in> nS))) nL iL = Some (q',x,nL')"
         by (metis prod_cases3)
-      then have "(select_inputs f q0 iL nL nS (Suc k) m) = select_inputs f q0 iL nL' (insert q' nS) k (m@[(q',x)])"
-        using None by auto
+      have "k = length nL'"
+        using find_remove_2_length[OF **] \<open>Suc k = length nL\<close> by simp
+
+      have "select_inputs f q0 iL nL nS m = select_inputs f q0 iL nL' (insert q' nS) (m @ [(q', x)])" 
+        using **
+        unfolding  \<open>nL = n # nL''\<close> select_inputs.simps None by auto
       
       have "length nL = Suc (length nL') \<and> distinct nL'"
         using find_remove_2_set(2,4,5)[OF **] \<open>distinct nL\<close>
         by (metis One_nat_def Suc_pred distinct_card distinct_remove1 equals0D length_greater_0_conv length_remove1 set_empty2 set_remove1_eq) 
-      then have "length (select_inputs f q0 iL nL' (insert q' nS) k (m@[(q',x)])) \<le> length m + Suc (length nL)"
-        using Suc.IH
+      then have "length (select_inputs f q0 iL nL' (insert q' nS) (m@[(q',x)])) \<le> length m + Suc (length nL)"
+        using Suc.hyps(1)[OF \<open>k = length nL'\<close>]
         by (metis add_Suc_shift length_append_singleton)
       then show ?thesis 
-        using \<open>(select_inputs f q0 iL nL nS (Suc k) m) = select_inputs f q0 iL nL' (insert q' nS) k (m@[(q',x)])\<close> by simp
+        using \<open>(select_inputs f q0 iL nL nS m) = select_inputs f q0 iL nL' (insert q' nS) (m@[(q',x)])\<close> by simp
     qed
   next
     case (Some a)
@@ -726,7 +823,7 @@ lemma select_inputs_q0_containment :
   assumes "f (q0,x) \<noteq> {}"
   and     "(\<forall> (y,q'') \<in> f (q0,x) . (q'' \<in> nS))"   
   and     "x \<in> set iL"
-shows "(\<exists> qx \<in> set (select_inputs f q0 iL nL nS k m) . fst qx = q0)" 
+shows "(\<exists> qx \<in> set (select_inputs f q0 iL nL nS m) . fst qx = q0)" 
 proof -
   have "find (\<lambda> x . f (q0,x) \<noteq> {} \<and> (\<forall> (y,q'') \<in> f (q0,x) . (q'' \<in> nS))) iL \<noteq> None"
     using assms unfolding find_None_iff by blast
